WIP: Semantics of timed formulas

PDDL-sema/States.thy
@@ -203,6 +203,60 @@ fun split_quant::"(('a \<times> 'b) list, 'c) GD \<Rightarrow> ('a \<times> 'b, 
 definition GD_sem::"(symbol \<Rightarrow> object) \<Rightarrow> ((variable \<times> type) list, symbol term atom) GD \<Rightarrow> bool option" where
   "GD_sem f \<phi> = ground_GD_sem (ground_GD f (replace_types_with_objects (split_quant \<phi>)))"
 
+fun remove_pref::"('a, 'b) pref_GD \<Rightarrow> ('a, 'b) GD" where
+  "remove_pref (pref_GD.Pref _ _) = GD.Not (GD.Bot)"
+| "remove_pref (pref_GD.GD \<phi>) = \<phi>"
+
+fun pref_GD_sem::"(symbol \<Rightarrow> object) \<Rightarrow> ((variable \<times> type) list, symbol term atom) pref_GD \<Rightarrow> bool option" where
+  "pref_GD_sem f (pref_GD.Pref _ _) = Some True"
+| "pref_GD_sem f (pref_GD.GD \<phi>) = GD_sem f \<phi>"
+
+lemma pref_GD_sem_alt[code]: "pref_GD_sem f x = GD_sem f (remove_pref x)"
+  by (cases x, auto simp: GD_sem_def)
+
+fun split_pref_GD_quant::"(('a \<times> 'b) list, 'c) pref_GD \<Rightarrow> ('a \<times> 'b, 'c) pref_GD" where
+  "split_pref_GD_quant (pref_GD.Pref p \<phi>) = (pref_GD.Pref p (split_quant \<phi>))"
+| "split_pref_GD_quant (pref_GD.GD \<phi>) = pref_GD.GD (split_quant \<phi>)"
+
+fun split_pre_GD_quant::"(('a \<times> 'b) list, 'c) pre_GD \<Rightarrow> ('a \<times> 'b, 'c) pre_GD" where
+  "split_pre_GD_quant (pre_GD.PrefGD \<phi>) = (pre_GD.PrefGD (split_pref_GD_quant \<phi>))"
+| "split_pre_GD_quant (pre_GD.ForAll vs \<phi>) = fold (\<lambda>v x. pre_GD.ForAll v x) vs (split_pre_GD_quant \<phi>)"
+| "split_pre_GD_quant (pre_GD.And x y) = pre_GD.And (split_pre_GD_quant x) (split_pre_GD_quant y)"
+
+abbreviation replace_pre_GD_types_with_objects where
+  "replace_pre_GD_types_with_objects \<equiv> map_pre_GD (\<lambda>(v, t). (v, ty_dom t)) id"
+
+fun ground_pref_GD::"(symbol \<Rightarrow> object) \<Rightarrow> (variable \<times> (object list), symbol term atom) pref_GD \<Rightarrow> (unit, object term atom) pref_GD" where
+  "ground_pref_GD f (pref_GD.Pref p \<phi>) = (pref_GD.Pref p (ground_GD f \<phi>))"
+| "ground_pref_GD f (pref_GD.GD \<phi>) = pref_GD.GD (ground_GD f \<phi>)"
+
+fun ground_pre_GD::"(symbol \<Rightarrow> object) \<Rightarrow> (variable \<times> (object list), symbol term atom) pref_GD \<Rightarrow> (unit, object term atom) pref_GD" where
+  
+
+fun pre_GD_sem::"(symbol \<Rightarrow> object) \<Rightarrow> ((variable \<times> type) list, symbol term atom) pre_GD \<Rightarrow> bool option" where
+  "pre_GD_sem f (pre_GD.PrefGD p) = pref_GD_sem f p"
+| "pre_GD_sem f (pre_GD.ForAll 
+
+(* preferences cannot be in conditions of conditional effects *)
+
+datatype ('x, 'a) pre_GD =
+  PrefGD "('x, 'a) pref_GD"
+  | ForAll 'x "('x, 'a) pre_GD"
+  | And 'x "('x, 'a) pre_GD"
+
+datatype ('x, atoms: 'a) timed_GD =
+  OverAll "('x, 'a) GD"
+| AtStart "('x, 'a) GD"
+| AtEnd "('x, 'a) GD"
+
+datatype ('x, atoms: 'a) pref_timed_GD =
+  Pref pref "('x, 'a) timed_GD"
+  | tGD "('x, 'a) timed_GD"
+
+datatype ('x, atoms: 'a) da_GD =
+  ForAll "'x" "('x, 'a) da_GD"
+| And "('x, 'a) da_GD" "('x, 'a) da_GD"
+| tGD "('x, 'a) pref_timed_GD"
 end
 
 end
