examples/example/example_dom.pddl
@@ -1,0 +1,25 @@
+(define 
+    (domain Example)
+    (:requirements :object-fluents)
+
+   
+    (:predicates
+        (p)
+        (q ?obj)
+    )
+
+    (:functions
+        (f ?obj) - object
+    )
+
+    (:action do
+        :parameters (?obj)
+        :precondition (= (f ?obj) (f ?obj))
+        :effect (p)
+    )
+
+    (:action do1
+        :parameters (?obj)
+        :effect (q (f ?obj))
+    )
+)
