examples/example/example_prob.pddl
@@ -1,0 +1,8 @@
+(define 
+    (problem ExampleProb)
+    (:domain ExampleDom)
+    (:objects obj1)
+    (:init (not p))
+
+    (:goal (p))
+)
