examples/example/example_prob1.pddl
@@ -1,0 +1,8 @@
+(define 
+    (problem ExampleProb1)
+    (:domain ExampleDom)
+    (:objects obj1)
+    (:init )
+
+    (:goal (q (f obj1)))
+)
